%%%%%%%%%%%%%%%%%%%%%%%%%%%%%%%%%%%%%%%%%%%%%%%%%%%%%%%%%%%%%%%%%%%%%%%%%%%%%%%%%%%%
%Do not alter this block of commands.  If you're proficient at LaTeX, you may include additional packages, create macros, etc. immediately below this block of commands, but make sure to NOT alter the header, margin, and comment settings here. 
\documentclass[12pt]{article}
 \usepackage{geometry} 
\usepackage{amsmath,amsthm,amssymb,amsfonts, enumitem, fancyhdr, color, comment, graphicx, environ,multicol}
\pagestyle{fancy}
%\setlength{\headheight}{65pt}
\newenvironment{problem}[2][Problem]{\begin{trivlist}
\item[\hskip \labelsep {\bfseries #1}\hskip \labelsep {\bfseries #2.}]}{\end{trivlist}}
\newenvironment{sol}
    {\emph{Solution:}
    }
    {
    \qed
    }
\specialcomment{com}{ \color{blue} \textbf{Comment:} }{\color{black}} %for instructor comments while grading
\NewEnviron{probscore}{\marginpar{ \color{blue} \tiny Problem Score: \BODY \color{black} }}
%%%%%%%%%%%%%%%%%%%%%%%%%%%%%%%%%%%%%%%%%%%%%%%%%%%%%%%%%%%%%%%%%%%%%%%%%%%%%%%%%





%%%%%%%%%%%%%%%%%%%%%%%%%%%%%%%%%%%%%%%%%%%%%
%Fill in the appropriate information below
\lhead{Student's name}  %replace with your name
\rhead{} %replace XYZ with the homework course number, semester (e.g. ``Spring 2019"), and assignment number.
%%%%%%%%%%%%%%%%%%%%%%%%%%%%%%%%%%%%%%%%%%%%%
\everymath{\displaystyle}

%%%%%%%%%%%%%%%%%%%%%%%%%%%%%%%%%%%%%%
%Do not alter this block.
\begin{document}
%%%%%%%%%%%%%%%%%%%%%%%%%%%%%%%%%%%%%%
\begin{center}
  {\Large \bf Formulas}
\end{center}

\begin{multicols}{2}
  {\large Exponents}
  \begin{description}
  \item $a^0=1$
  \item $ a^m\cdot a^n = a^{m+n}$
  \item $ \frac{a^n}{a^m} = a^{n-m} $
  \item $ (a^n)^m = a^{mn} $
  \item $ (ab)^n = a^nb^b $
  \item $ \left( \frac{a}{b} \right)^n = \frac{a^n}{b^n}$
  \item $ \left(\frac{a}{b}\right)^{-n} = \left(\frac{b}{a}\right)^n $
  \end{description}
    
  {\large Product/factors}
  \begin{description}
  \item $(a+b)^2 = a^2 + 2ab + b^2$
  \item $(a-b)^2 = a^2 - 2ab + b^2  $
  \item $ a^2 - b^2 = (a-b)(a+b) $
  \item $ a^3 + b^3 = (a+b)(a^2 - ab + b^2) $
  \item $ a^3 - b^3 = (a-b)(a^2 + ab + b^2) $
  \end{description}
  
  {\large Radicals}
  \begin{description}
  \item $ \sqrt[n]{xy} = \sqrt[n]{x}\sqrt[n]{y}$
  \item $\sqrt[n]{\frac{x}{y}} = \frac{\sqrt[n]{x}}{\sqrt[n]{y}}$
  \item $ x^{\frac{m}{n}} = \sqrt[n]{x^m} = (\sqrt[n]{x})^m $
  \end{description}

  {\large Square Root Property}
  
  If $X^2 = k$ and $k \geq 0$ then $X = \pm k$.

  \vspace{.25in}
  {\large Quadratic formula}

  $\Delta = b^2 -4ac$, $\displaystyle \frac{-b\pm\sqrt{\Delta}}{2a}$

  \vspace{.25in}
  {\large{Parabolas}}

  $x$-coordinate of vertex $x_v=\displaystyle\frac{-b}{2a}$

  \vspace{.25in}
  {\large{lines}}

  \begin{description}
  \item General formula $Ax+By=C$
  \item Standard formula $y = mx+b$
  \item Point slope formula $y-y_1 = m(x-x_1)$
  \item slope $m=\displaystyle\frac{y_2-y_1}{x_2-x_1}$
  \end{description}

  \vspace{.25in}
  {\large{distance and midpoint}}

  \begin{description}
  \item $d=\sqrt{(x_2-x_1)^2+(y_2-y_1)^2}$
    \item $\displaystyle\left(\frac{x_1+x_2}{2},\frac{y_1+y_2}{2}\right)$
  \end{description}

  \vspace{.25in}
  {\large{Logarithms}}

  \begin{description}
  \item $\log_b y = x$ if and only if $b^x=y$
  \item $\log_a a=1$, $\log_a 1 = 0$, $\log_a a^x=x$
  \item $ \displaystyle \log_b y = \frac{\log y}{\log b}$
  \end{description}
  

  
  
  
  
  
\end{multicols}


%% \begin{problem}{1}
%%   Evaluate each expression
%% \begin{multicols}{2}
%%   \begin{enumerate}[label=\roman*)]
%%   \item  $ -9^{1/2}$
%%   \item $27^{1/3}$
%%   \item $ (-64)^{1/3}$
%%   \item $(-27)^{4/3}$
%%   \item $125^{-2/3}$
%%   \item $8^{-4/3}$
%%   \item $ \left(\frac{1}{4}\right)^{1/2}$
%%   \item $ \left( \frac{4}{9} \right)^{3/2}$
%%     \item $\left(-\frac{8}{27}\right)^{2/3}$
%%     \item $7\sqrt{288}$
%%   \end{enumerate}
%% \end{multicols}
%% \end{problem}
%\begin{sol}
%Write your solution here.
%\end{sol}

%Do not alter anything below this line.
\end{document}
